theories/iris_use.v
@@ -1,13 +1,28 @@
 (** Example of Iris usage **)
 (* (C) J. Pichon, M. Bodin - see LICENSE.txt *)
 
+From mathcomp Require Import eqtype.
 From iris.program_logic Require Import language.
 From iris.proofmode Require Import tactics.
 From iris.program_logic Require Export weakestpre.
-Require Export operations iris.
+Require Export host operations iris.
 Set Default Proof Using "Type". (* what is this? *)
 
 Close Scope byte_scope.
+
+Section Host.
+
+Variable host_function : eqType.
+
+Let host := host host_function.
+Let expr := expr host_function.
+
+Variable host_instance : host.
+
+Let wasm_mixin : LanguageMixin _ _ _ := wasm_mixin host_instance.
+
+Canonical Structure wasm := Language wasm_mixin.
+
 
 Record loc := { loc_car : Z }.
 Instance loc_eq_decision : EqDecision loc.
@@ -35,11 +50,11 @@ Class heapG Σ := HeapG {
 }.
 
 Instance heapG_irisG `{!heapG Σ} : irisG wasm_lang Σ := {
-  iris_invG := heapG_invG;
-  state_interp σ κs _ := True%I
-(*    (gen_heap_ctx σ.(heap) ∗ proph_map_ctx κs σ.(used_proph_id))%I*);
-  fork_post _ := True%I;
-                                                       }.
+    iris_invG := heapG_invG;
+    state_interp σ κs _ := True%I
+      (* (gen_heap_ctx σ.(heap) ∗ proph_map_ctx κs σ.(used_proph_id))%I*);
+    fork_post _ := True%I;
+  }.
 
 Definition xx i := (ConstInt32 (Wasm_int.int_of_Z i32m i)).
 
@@ -52,11 +67,13 @@ Lemma wp_nil `{!heapG Σ} (s : stuckness) (E : coPset) (Φ : iProp Σ) :
   Φ -∗ WP ([] : expr) @ s ; E {{ fun v => Φ }}%I.
 Proof.
   iIntros "H".
-  
 Admitted. (* TODO *)
 
 Lemma wp_seq `{!heapG Σ} (s : stuckness) (E : coPset) (Φ : val -> iProp Σ) (es1 es2 : expr) :
-  WP (es2 : expr) @ s ; E {{ fun v => WP (es1 : expr) @ s ; E {{ fun v' => Φ (v ++ v') }}%I }}%I -∗ WP ((es1 ++ es2) : expr) @ s ; E {{ Φ }}%I.
+  WP (es2 : expr) @ s ; E {{ fun v =>
+   WP (es1 : expr) @ s ; E {{ fun v' =>
+     Φ (v ++ v') }}%I }}%I
+  -∗ WP ((es1 ++ es2) : expr) @ s ; E {{ Φ }}%I.
 Proof.
   elim: es1.
   { iIntros "H".
@@ -69,7 +86,8 @@ Proof.
 Admitted. (* TODO *)
 
 Lemma wp_val `{!heapG Σ} (s : stuckness) (E : coPset) (Φ : val -> iProp Σ) (v0 : value) (es : expr) (v : val) :
-  WP es @ s ; E {{ v, (Φ (v0 :: v)) }}%I -∗ WP (((Basic (EConst v0)) :: es) : expr) @ s ; E {{ v, Φ v }}%I.
+  WP es @ s ; E {{ v, (Φ (v0 :: v)) }}%I
+  -∗ WP (((Basic (EConst v0)) :: es) : expr) @ s ; E {{ v, Φ v }}%I.
 Proof.
 Admitted. (* TODO *)
 
@@ -83,4 +101,6 @@ Proof.
   simpl.
   (* FIXME: iApply. *)
 Admitted.
+
+End Host.
 
